				<exercises>
				<p><exercise><!-- xml:id="ex-" --><!-- Replacement for Poole's Section 2.1, Exercise 35 and 37-->
						<statement>
							<aside><p> (Source: <xref ref="ref-KN"/>, Section 1.1, Exercise 1.1.19.) </p></aside>
							Find the solution of each of the following systems of linear equations using Gauss-Jordan elimination and augmented matrices.
							 <ol label="[a]" cols="2">
							 	<li>
							 		<md>
										<mrow> 
											x - 3y \amp = 1
										</mrow>
										<mrow>
											2x - 7y \amp = 3
										</mrow>
									</md>
								</li>
								<li>
									<md>
										<mrow> 
											x - 2y \amp = 1
										</mrow>
										<mrow>
											3x + 4y \amp = -1
										</mrow>
									</md>
								</li>
								<li>
									<md>
										<mrow>
											2x - 3y \amp = -1
										</mrow>
										<mrow>
											3x + 4y \amp = 2
										</mrow>
									</md>
								</li>
								<li>
									<md>
										<mrow> 
											3x + 4y \amp = 1
										</mrow>
										<mrow>
											4x + 5y \amp = -3
										</mrow>
									</md>
								</li>
							</ol>
	 						</statement>
	 					<hint>
	 						Use row operations to reduce the augmented matrix into a triangular form, such as the following.
	 							<me>
								\matr{cc|c} {  * \amp  * \amp  *\\
									0 \amp  * \amp  * }							
							</me>							
							Then, use back substition to find a solution as in <xref ref = "exercise-back-substitution"/>. 
	 						</hint>
	 						<answer>
	 							 <ol label="[a]" cols="2">
							 	<li>
							 		<m> x =- 2, y = -1 </m>
								</li>
								<li>
									<m> x = \frac{1}{5}, y = -\frac{2}{5} </m>
								</li>
								<li>
									<m> x = -7, y = 13 </m>
								</li>
								<li>
									<m> x = -17, y = 13 </m>
								</li>
							</ol>
						</answer> 
						<solution>
							<ol label="[a]">
							<li>
								First, we write the augmented matrix for the system of linear equations.
								
								<md>
									<mrow>
									\matr{cc|c}{1\amp -3\amp 1\\ 2 \amp -7 \amp 3}
									</mrow>
								</md>

								Next, we  put this augmented matrix into a triangular form by eliminating the lower left hand entry.   Subtracting (2) times row 1 from row 2.
								<md>
								<mrow>
								\matr{cc|c}{1\amp -3\amp 1\\ 0\amp -1 \amp 1} \amp \hspace{.25in} R_2-2R_1 \to R_2
								</mrow>
								</md>
								This corresponds to the system of equations, 
								<md>
										<mrow> 
											x -3y \amp = 1
										</mrow>
										<mrow>
											  -y \amp = 1
										</mrow>
									</md>
								At this point, we may back substitute in order to solve the system.  Substituting <m> y = -1 </m> into the first equation gives <m> x - 3(-1) =1 .</m>   Solving this equation for <m> x </m> yields <m> x = -2 </m>.   Therefore, the solution to the system is <m> x = -2, y = -1 </m>.
 							</li>
 							<li>
								The augmented matrix to the system is given by,
								
								<md>
									<mrow>
									\matr{cc|c}{1\amp -2\amp 1\\ 3 \amp 4 \amp -1}.
									</mrow>
								</md>

								Next, we  put this augmented matrix into a triangular form by eliminating the lower left hand entry.   This is done by subtracting (3) times row 1 from row 2.
								<md>
									<mrow>
									\matr{cc|c}{1\amp -2\amp 1\\ 0\amp 10 \amp -4} \amp \hspace{.25in}  R_2 -3R_1 \to R_2
									</mrow>
								</md>
								This corresponds to the system of equations, 
								<md>
									<mrow> 
									x -2y \amp = 1
									</mrow>
									<mrow>
									10y \amp = -4
									</mrow>
								</md>
							We may back substitute in order to solve the system.  We have that <m> y =-\frac{2}{5} </m> from the second equation.  Substituting <m> y =-\frac{2}{5} </m>  into the first equation gives <m> x - 2\left(-\frac{2}{5}\right) =1 .</m>   Solving this equation for <m> x </m> yields <m> x = \frac{1}{5} </m>.   Therefore, the solution to the system is <m> x = \frac{1}{5} , y = -\frac{2}{5} </m>.
 							</li>
 							<li>
								The augmented matrix to the system is given by,
								
								<md>
									<mrow>
									\matr{cc|c}{2\amp -3\amp -1\\ 3 \amp 4 \amp 2}.
									</mrow>
								</md>

								Next, we  put this augmented matrix into a triangular form by eliminating the lower left hand entry.   This is done by subtracting <m> \left(\frac{3}{2}\right) </m> times row 1 from row 2.   
								<md>
								<mrow>
								\matr{cc|c}{2\amp -3\amp -1\\ 0\amp \frac{17}{2} \amp \frac{7}{2} }\amp \hspace{.25in} R_2 - \frac{3}{2}R_1 \to R_2
								</mrow>
								</md>
								This corresponds to the system of equations, 
								<md>
										<mrow> 
											2x -3y \amp = -1
										</mrow>
										<mrow>
										  \frac{17}{2}y \amp = \frac{7}{2}
										</mrow>
									</md>
							We may back substitute in order to solve the system.  We have that <m> y =\frac{7}{17} </m> from the second equation.  Substituing <m> y =\frac{7}{17}</m>  into the first equation gives <m> 2x - 3\left(\frac{7}{17}\right) =-1 .</m>   Solving this equation for <m> x </m> yields <m> x = \frac{2}{17} </m>.   Therefore, the solution to the system is <m> x = \frac{2}{17} , y = \frac{7}{17} </m>.
 							</li>
 							<li>
								The augmented matrix to the system is given by,
								
								<md>
									<mrow>
									\matr{cc|c}{3\amp 4\amp 1\\ 4 \amp 5 \amp -3}.
									</mrow>
								</md>

								Next, we  put this augmented matrix into a triangular form by eliminating the lower left hand entry.   This is done by subtracting <m> \left(\frac{4}{3}\right) </m> times row 1 from row 2.   
								<md>
								<mrow>
								\matr{cc|c}{3\amp 4\amp 1\\ 0 \amp -\frac{1}{3} \amp -\frac{13}{3}} \amp \hspace{.25in} R_2 - \frac{4}{3}R_1 \to R_2
								</mrow>
								</md>
								This corresponds to the system of equations, 
								<md>
										<mrow> 
											3x +4y \amp = 1
										</mrow>
										<mrow>
											 -\frac{1}{3}y \amp = -\frac{13}{3}
										</mrow>
									</md>
							We may back substitute in order to solve the system.  We have that <m> y =13 </m> from the second equation.  Substituing <m> y =13</m>  into the first equation gives <m> 3x + 4(13) =1 .</m>   Solving this equation for <m> x </m> yields <m> x = -17 </m>.   Therefore, the solution to the system is <m> x = -17 , y = 13 </m>.
 							</li>
							</ol>
						</solution> 
						
					</exercise></p>
					<p><exercise><!-- xml:id="ex-" -->
						<statement>
							<aside><p> (Source: <xref ref="ref-PS"/>, Section 1.3, Exercise 1.3.4.) </p></aside>
							Do the three planes, <m>x+y-3z=2</m>, <m>2x+y+z=1</m>, and <m>3x + 2y-2z =0</m> have a common point of intersection? If so, find one and if not, tell why there is no such point.  Note that a point of intersection is a point that satisfies all three equations.
						</statement>
						<hint>
							The three planes give a system of three equations.  A solution to the system will be the common point of intersection. 
						</hint>
						<hint>
							To solve the system of three equations, transform the system into one that exhibits the triangular structure of <xref ref = "exercise-back-substitution"/>. 
						</hint>
						
						<answer>
						The three planes do not have a common point of intersection because the system of equations is <em> inconsistent </em>, it has no solution.
						</answer>
						<solution>
							We start with the system of three equations. 
								<md>
										<mrow>
											x + y -3z \amp = \amp 2
										</mrow>
										<mrow>											 
											 2x + y +z \amp = \amp 1
										</mrow>
										<mrow>											 
											3x  + 2y -2z \amp = \amp 0
										</mrow>
									</md>
							To transform this system into one that exhibits a triangular structure we must first eliminate the variable <m> x </m> from the third equation.  We may do to this by subtracting (3) times the first row from the third row.  
								<md>
										<mrow>
											x + y -3z \amp =  2 \amp \hspace{.2in}
										</mrow>
										<mrow>											 
											 2x + y +z \amp = 1 \amp
										</mrow>
										<mrow>											 
											 -y +7z \amp = -6 \amp R_3-3R1  
										</mrow>
									</md>
							Next, we can eliminate the variable <m> x </m> from the second equation.  We may do this by subtracting (2) times the first row from the second row. 

									<md>
										<mrow>
											x + y -3z \amp =  2 \amp \hspace{.2in}
										</mrow>
										<mrow>											 
											  -y +7z \amp = -3 \amp  R_2-2R_1
										</mrow>
										<mrow>											 
											 -y +7z \amp = -6 \amp
										</mrow>
									</md>

							Lastly, notice that subtracting the last two equations gives a contradiction, 0 is certainly not equal to -3.  
							
								<md>
										<mrow>
											x + y -3z \amp =  2 \amp \hspace{.2in}
										</mrow>
										<mrow>											 
											  -y +7z \amp = -3 \amp 
										</mrow>
										<mrow>											 
											 0\amp = -3 \amp  R_3 - R_2
										</mrow>
									</md>	

									Therefore, the system does not have a solution and so the three planes do not have a common point of intersection.
								</solution> 
						
					</exercise></p>
					<p><exercise><!-- xml:id="ex-" -->
						<statement>
							<aside><p> (Source: <xref ref="ref-KN"/>, Section 1.1, Exercise 1.1.15.) </p></aside>
							Find a quadratic <m>a +bx +cx^2</m> such that the graph of <m>y = a + bx + cx^2</m> contains the points <m>(-1,6)</m>, <m>(2,0)</m>, and <m>(3,2)</m>.	 
						</statement>
						<hint> For some fixed value of <m>a,b </m> and <m> c, </m> each of the points,<m>(-1,6)</m>, <m>(2,0)</m>, and <m>(3,2)</m>, is a solution to the quadratic equation <m>y = a + bx + cx^2</m>.
						</hint> 
						<answer>
							<me> 2-3x+x^2 </me>
						</answer> 
						<solution>
							Each of the points,<m>(-1,6)</m>, <m>(2,0)</m>, and <m>(3,2)</m>, is a solution to the quadratic equation <m>y = a + bx + cx^2</m>, which means that each of those values of <m> x </m> and <m> y </m> satisfies the equation.  This creates a system of three equations with three variables <m> a,b </m> and <m> c </m>.
								<md>
										<mrow> 
											a -b +c \amp = 6
										</mrow>
										<mrow>
											 a + 2b + 4c \amp = 0
										</mrow>
										<mrow>
											 a + 3b + 9c  \amp = 2
										</mrow>
									</md>
							Rewriting this system as an augmented matrix,
							<me>
								\matr{ccc|c}{1\amp -1\amp 1\amp 6\\ 1 \amp 2 \amp 4 \amp 0 \\ 1 \amp 3 \amp 9 \amp 2}
							</me>
							At this point, we may perform row operations to transform this augmented matrix into a triangular form.  Our first task is to eliminate the lower left term.  We may do this by subtracting row 2 from row 1. 

							<md>
								<mrow>
								\matr{ccc|c}{1\amp -1\amp 1\amp 6\\ 1 \amp 2 \amp 4 \amp 0 \\ 0 \amp 1 \amp 5 \amp 2} \amp \hspace{.25in} R_3 - R_2 \to R_3
							</mrow>
							</md>
							Next, we may eleminate the left most entry of the middle row by subtracting row 1 from row 2. 
							<md>
							<mrow>
								\matr{ccc|c}{1\amp -1\amp 1\amp 6\\ 0 \amp 3 \amp 3 \amp -6 \\ 0 \amp 1 \amp 5 \amp 2} \amp \hspace{.25in} R_2 - R_1 \to R_2
							</mrow>
							</md>
							Next, we simplify the second row by multiplying by <m> \frac{1}{3} .</m>  This step is not necessary for getting the matrix to triangular form, it just makes things simpler.
							<md>
							<mrow>
								\matr{ccc|c}{1\amp -1\amp 1\amp 6\\ 0 \amp 1 \amp 1 \amp -2 \\ 0 \amp 1 \amp 5 \amp 2} \amp \hspace{.25in} \frac{1}{3}R_2 \to R_2
							</mrow>
							</md>
							Our last step to write this augmented matrix in triangular form is to eliminate the middle term of the last row.  We may do this by subtracting row 2 from row 3. 
							<md>
							<mrow>
								\matr{ccc|c}{1\amp -1\amp 1\amp 6\\ 0 \amp 1 \amp 1 \amp -2 \\ 0 \amp 0 \amp 4 \amp 4} \amp \hspace{.25in} R_3-R_3 \to R_3
							</mrow>
							</md>
							Now, we can solve the system by back substitution. 
							<md>
										<mrow> 
											a -b +c \amp = 6
										</mrow>
										<mrow>
											 b + c \amp = -2
										</mrow>
										<mrow>
											 4c \amp = 4
										</mrow>
									</md>  
							Substitution <m> c =1 </m> into the second equation gives <m> b = -3. </m> Finally, substituting both <m> b </m> and <m> c </m> into the first equation and solving for <m> a, </m> yields the final solution <m> a = 2, b = -3, c = 1 </m>.  Just for fun, we may graph the parabola <m> y = 2 -3 x + x^2 </m> to verify that it indeed does contain the points given.    
							<image source = "chp2-1q9.png"/>
						</solution> 
					</exercise></p>
				</exercises>
		